
\subsection*{1b}

For $M=1$ the equation becomes:

\begin{equation}
    \beta_1 \sum_{n=1}^{N} \mathbbm{1}_{u_{1,n}(x) = u_{1,n}(x')}
\end{equation}

We map every entery of x to:

\begin{equation}
g(x_i) = \begin{pmatrix}
    \mathbbm{1}_{x_i = A} \\
    \mathbbm{1}_{x_i = C} \\
    \mathbbm{1}_{x_i = G} \\
    \mathbbm{1}_{x_i = T}
\end{pmatrix}
\end{equation}
That means an A is mapped to $[1, 0, 0, 0]$ and analogously G is mapped to $[0, 0, 1, 0]$.

The feature map is a concatenation of all $g(x_i)$ vectors and we have to account
to the factor $\beta_1$:
\begin{equation}
\phi(x) = \sqrt{\beta_1} \begin{pmatrix}
    g(x_1) \\
    \ldots \\
    g(x_N)
\end{pmatrix}
\end{equation}

The the dot product of two feature maps is:
\begin{align}
    \phi(x)^T \phi(x') &=
       \sqrt{\beta_1} \begin{pmatrix} g(x_1) & \ldots & g(x_N) \end{pmatrix}
       \sqrt{\beta_1}
       \begin{pmatrix}
            g(x'_1) \\
            \ldots \\
            g(x'_N)
       \end{pmatrix} \\
       & = \beta_1 \sum_{n=1}^{N} g(x_n)^T  g(x'_n)
\end{align}

And here, we observe that $g(x_n)^T g(x'_n) = 1$ iff $u_{1,n}(x) = u_{1,n}(x')$.
