\section*{Task 3}

\subsection*{a}

\begin{gather*}
\forall_{j=1}^d : x_j = 0.1(tanh(\sum_{i=1}^d x_i w_{ij} + b_j) - x_j) \\
\end{gather*}
Eulers discretization of $y'(t) = f(t,y(t))$ is: 
\begin{gather*}
y^{(t)} = y^{(t-1)} + hf(t-1, y^{(t-1)}) \\
\end{gather*}
We have $h=1$: 
\begin{gather*}
x_j^{(t)} = x_j^{(t-1)} + 0.1(tanh(\sum_{i=1}^d x_i^{(t-1)} w_{ij} + b_j) - x_j^{(t-1)}) \\
= 0.9 x_j^{(t-1)} + 0.1(tanh(\sum_{i=1}^d x_i^{(t-1)} w_{ij} + b_j))
\end{gather*}


\subsection*{b}

\subsection*{c}
\begin{gather*}
\frac{\partial x_j^{(t)}}{\partial x_j^{(t-1)}} = 0.9 + 0.1(1 - tanh^2(\sum_{i=1}^d x_i^{(t-1)} w_{ij} + b_j) w_{jj}) \\
= 0.9 + 0.1 - 0.1 tanh^2(\sum_{i=1}^d x_i^{(t-1)} w_{ij} + b_j) w_{jj} \\
= 1 - 0.1 tanh^2(\sum_{i=1}^d x_i^{(t-1)} w_{ij} + b_j) w_{jj}
\end{gather*}
For $k \neq j$: 
\begin{gather*}
\frac{\partial x_k^{(t)}}{\partial x_j^{(t-1)}} = 0.1(1 - tanh^2(\sum_{i=1}^d x_i^{(t-1)} w_{ik} + b_k) w_{jk}) \\
= 0.1 - 0.1 w_{jk} tanh^2(\sum_{i=1}^d x_i^{(t-1)} w_{ik} + b_k)
\end{gather*}

\subsection*{d}

\begin{gather*}
\frac{\partial x_j^{(t)}}{\partial w_{kj}} = 0.1(1 - tanh^2(\sum_{i=1}^d x_i^{(t-1)} w_{ij} + b_j) x_k^{(t-1)}) \\
= 0.1 - 0.1 x_k^{(t-1)} tanh^2(\sum_{i=1}^d x_i^{(t-1)} w_{ij} + b_j) \\
\frac{\partial x_j^{(t)}}{\partial w_{kl}} = 0 \ for \ l \neq j
\end{gather*}

\begin{gather*}
\frac{\partial x_j^{(t)}}{\partial b_j} = 0.1 + 0.1 tanh^2(\sum_{i=1}^d x_i^{(t-1)} w_{ij} + b_j) \\
\frac{\partial x_j^{(t)}}{\partial b_k} = 0 \ for \ k \neq j
\end{gather*}



