\section*{Task 2}

\subsection*{i}

\begin{gather*}
\epsilon = |\vec{x}  - \sum_j w_j \vec{\eta_j}|^2 \\
\epsilon = |\underbrace{\sum_j w_j}_{=1} \vec{x} -  \sum_j w_j \vec{\eta_j}|^2 \\
\epsilon = |\sum_j w_j (\vec{x} - \vec{\eta_j})|^2 \\
\epsilon = (\sum_j w_j (\vec{x} - \vec{\eta_j})) (\sum_k w_k (\vec{x} - \vec{\eta_k})) \\
\epsilon = \sum_j \sum_k w_j w_k  (\vec{x} - \vec{\eta_j}) (\vec{x} - \vec{\eta_k}) \\
\epsilon = \sum_{j,k} w_j w_k C_{jk} \\
\epsilon = \sum_j w_j \sum_k C_{jk} w_k \\
\epsilon = \sum_j w_j (C w)_j
\end{gather*}
where $(C w)_j = \sum_j C_{kj} w_j$ and $C_{kj} = (\vec{x} - \vec{\eta_k}) (\vec{x} - \vec{\eta_j}) = (\vec{x} - \vec{\eta_j}) (\vec{x} - \vec{\eta_k}) = C_{jk}$
\begin{gather*}
\epsilon = \vec{w}^TC\vec{w} \\
\end{gather*}

\subsection*{ii}

\begin{gather*}
L(w,\lambda) = w^T Cw + \lambda(w^T 1 - 1) \\
\frac{\partial L}{\partial \lambda} = w^T  -1 \\
\frac{\partial L}{\partial w_i} = \frac{\partial}{\partial w_i} \\
\end{gather*}
\todo[inline]{Mathbbm is not working}
\todo[inline]{Finish this task}
\subsection*{iii}

\todo[inline]{Finish this task}

\clearpage
